add selection benchmarks

Selection/benchmarks/results/_lfind_selection_lemma_le_trans_IN_select_smallest/extract.ml
@@ -1,0 +1,17 @@
+
+  module SS = Set.Make(String)
+  let values = ref SS.empty
+    
+  let write_to_file value=
+    let oc = open_out_gen [Open_append; Open_creat] 0o777 "/home/anabrendel/lfind/vfa-benchmarks/Selection/benchmarks/sources/_lfind_selection_lemma_le_trans_IN_select_smallest/examples_Selection.txt" in
+    if not(SS.mem value !values) then 
+      (
+        values := SS.add value !values;
+        Printf.fprintf oc "%s\n"  value;
+      );
+    close_out oc; ()
+  
+  let print n nstr=
+    write_to_file (String.of_seq (List.to_seq nstr));
+    (n)
+    
