Selection/benchmarks/results/_lfind_selection_lemma_Permutation_sym_IN_cons_of_small_maintains_sortt/lfind_quickchick_generator.v
@@ -1,0 +1,28 @@
+Load LFindLoad.
+
+From lfind Require Import LFind.
+From VFA Require Import Perm.
+From QuickChick Require Import QuickChick.
+Load LFindLoad.
+From vfa_benchmark Require Import Selection.
+
+Lemma lfind_state   (a : nat) (l : list nat) (y : nat) (bl : list nat) : @Permutation nat ?l bl.
+Admitted.
+
+From QuickChick Require Import QuickChick.
+QCInclude "/home/anabrendel/lfind/vfa-benchmarks/Selection/benchmarks/sources/_lfind_selection_lemma_Permutation_sym_IN_cons_of_small_maintains_sortt/".
+QCInclude ".".
+Extract Constant defNumTests => "50".
+
+Require Import decide.
+
+Open Scope string_scope.
+
+Parameter print : list nat -> string -> list nat.
+Extract Constant print => "Extract.print".
+Definition collect_data (a : nat) (l : list nat) (y : nat) (bl : list nat) :=
+ let lfind_var := "a:" ++ "(" ++ show a ++ ")"++ "`" ++"l:" ++ "(" ++ show l ++ ")"++ "`" ++"y:" ++ "(" ++ show y ++ ")"++ "`" ++"bl:" ++ "(" ++ show bl ++ ")"
+ in let lfind_v := print bl lfind_var
+ in lfind_state a l y lfind_v.
+QuickChick collect_data.
+Success.
