Selection/benchmarks/results/_lfind_selection_lemma_list_has_length_IN_selsortt_is_correct/lfind_quickchick_generator.v
@@ -1,0 +1,28 @@
+Load LFindLoad.
+
+From lfind Require Import LFind.
+From VFA Require Import Perm.
+From QuickChick Require Import QuickChick.
+Load LFindLoad.
+From vfa_benchmark Require Import Selection.
+
+Lemma lfind_state   (al : list nat) : @ex nat (fun x : nat => @eq nat (@list_length nat al) x).
+Admitted.
+
+From QuickChick Require Import QuickChick.
+QCInclude "/home/anabrendel/lfind/vfa-benchmarks/Selection/benchmarks/sources/_lfind_selection_lemma_list_has_length_IN_selsortt_is_correct/".
+QCInclude ".".
+Extract Constant defNumTests => "50".
+
+Require Import decide.
+
+Open Scope string_scope.
+
+Parameter print : list nat -> string -> list nat.
+Extract Constant print => "Extract.print".
+Definition collect_data (al : list nat) :=
+ let lfind_var := "al:" ++ "(" ++ show al ++ ")"
+ in let lfind_v := print al lfind_var
+ in lfind_state  lfind_v.
+QuickChick collect_data.
+Success.
