Selection/benchmarks/results/_lfind_selection_lemma_select_exists_IN_selsort_sorted/lfind_quickchick_generator.v
@@ -1,0 +1,30 @@
+Load LFindLoad.
+
+From lfind Require Import LFind.
+From VFA Require Import Perm.
+From QuickChick Require Import QuickChick.
+Load LFindLoad.
+From vfa_benchmark Require Import Selection.
+
+Lemma lfind_state   (n : nat) (al : list nat) : sorted
+  (let (y, r') := select n0 al in
+   @cons nat y (selsort r' (@list_length nat al))).
+Admitted.
+
+From QuickChick Require Import QuickChick.
+QCInclude "/home/anabrendel/lfind/vfa-benchmarks/Selection/benchmarks/sources/_lfind_selection_lemma_select_exists_IN_selsort_sorted/".
+QCInclude ".".
+Extract Constant defNumTests => "50".
+
+Require Import decide.
+
+Open Scope string_scope.
+
+Parameter print : list nat -> string -> list nat.
+Extract Constant print => "Extract.print".
+Definition collect_data (n : nat) (al : list nat) :=
+ let lfind_var := "n:" ++ "(" ++ show n ++ ")"++ "`" ++"al:" ++ "(" ++ show al ++ ")"
+ in let lfind_v := print al lfind_var
+ in lfind_state n lfind_v.
+QuickChick collect_data.
+Success.
