Selection/benchmarks/results/_lfind_selection_lemma_select_smallest_IN_selsort_sorted/lfind_quickchick_generator.v
@@ -1,0 +1,28 @@
+Load LFindLoad.
+
+From lfind Require Import LFind.
+From VFA Require Import Perm.
+From QuickChick Require Import QuickChick.
+Load LFindLoad.
+From vfa_benchmark Require Import Selection.
+
+Lemma lfind_state   (n0 : nat) (n : nat) (al : list nat) (x : nat) (x0 : list nat) : le_all x x0.
+Admitted.
+
+From QuickChick Require Import QuickChick.
+QCInclude "/home/anabrendel/lfind/vfa-benchmarks/Selection/benchmarks/sources/_lfind_selection_lemma_select_smallest_IN_selsort_sorted/".
+QCInclude ".".
+Extract Constant defNumTests => "50".
+
+Require Import decide.
+
+Open Scope string_scope.
+
+Parameter print : list nat -> string -> list nat.
+Extract Constant print => "Extract.print".
+Definition collect_data (n0 : nat) (n : nat) (al : list nat) (x : nat) (x0 : list nat) :=
+ let lfind_var := "n0:" ++ "(" ++ show n0 ++ ")"++ "`" ++"n:" ++ "(" ++ show n ++ ")"++ "`" ++"al:" ++ "(" ++ show al ++ ")"++ "`" ++"x:" ++ "(" ++ show x ++ ")"++ "`" ++"x0:" ++ "(" ++ show x0 ++ ")"
+ in let lfind_v := print x0 lfind_var
+ in lfind_state n0 n al x lfind_v.
+QuickChick collect_data.
+Success.
