Selection/benchmarks/results/_lfind_selection_lemma_selsort_perm_IN_selection_sort_perm/lfind_eval.v
@@ -1,0 +1,13 @@
+Load LFindLoad.
+From lfind Require Import LFind.
+From VFA Require Import Perm.
+From vfa_benchmark Require Import Selection.
+
+Set Printing Depth 1000.
+Unset Printing Notations.
+Set Printing Implicit.
+
+Definition lfind_eval (l : list nat) :=
+@length nat l.
+
+Compute lfind_eval ((nil)).
