Selection/benchmarks/results/_lfind_selection_lemma_selsort_sorted_IN_selection_sort_sorted/lfind_conj4.v
@@ -1,0 +1,18 @@
+Load LFindLoad.
+
+From lfind Require Import LFind.
+From VFA Require Import Perm.
+From QuickChick Require Import QuickChick.
+Load LFindLoad.
+From vfa_benchmark Require Import Selection.
+
+From QuickChick Require Import QuickChick.
+QCInclude "/home/anabrendel/lfind/vfa-benchmarks/Selection/benchmarks/sources/_lfind_selection_lemma_selsort_sorted_IN_selection_sort_sorted/".
+QCInclude ".".
+Extract Constant defNumTests => "50".
+
+Require Import decide.
+
+Lemma conj4: forall (al : list nat), sorted (selsort al (@length nat al)).
+Admitted.
+QuickChick conj4.
