Selection/benchmarks/results/_lfind_selection_lemma_selsortt_perm_IN_selsortt_is_correct/Selection.v
@@ -1,0 +1,284 @@
+(** * Selection:  Selection Sort *)
+(* Some proofs from: https://github.com/kolya-vasiliev/verified-functional-algorithms-2019/blob/master/Selection.v *)
+
+Load LFindLoad.
+From lfind Require Import LFind.
+Unset Printing Notations.
+Set Printing Implicit.
+
+Set Warnings "-notation-overridden,-parsing,-deprecated-hint-without-locality".
+From VFA Require Import Perm.
+Hint Constructors Permutation : core.
+From Coq Require Export Lists.List.  (* for exercises involving [List.length] *)
+
+Definition list_length {T} (l : list T) := List.length l.
+
+(* ################################################################# *)
+(** * The Selection-Sort Program  *)
+Fixpoint select (x: nat) (l: list nat) : nat * list nat :=
+  match l with
+  | [] => (x, [])
+  | h :: t =>
+    if x <=? h
+    then let (j, l') := select x t
+         in (j, h :: l')
+    else let (j, l') := select h t
+         in (j, x :: l')
+  end.
+
+Fixpoint selsort (l : list nat) (n : nat) : list nat :=
+  match l, n with
+  | _, O => []  (* ran out of fuel *)
+  | [], _ => []
+  | x :: r, S n' => let (y, r') := select x r
+                  in y :: selsort r' n'
+end.
+
+Definition selection_sort (l : list nat) : list nat :=
+  selsort l (length l).
+  
+(* ################################################################# *)
+(** * Proof of Correctness *)
+
+Inductive sorted: list nat -> Prop :=
+ | sorted_nil: sorted []
+ | sorted_1: forall i, sorted [i]
+ | sorted_cons: forall i j l, i <= j -> sorted (j :: l) -> sorted (i :: j :: l).
+
+Hint Constructors sorted : core.
+
+Definition is_a_sorting_algorithm (f: list nat -> list nat) := forall al,
+    Permutation al (f al) /\ sorted (f al).
+
+Lemma select_perm: forall x l y r, select x l = (y, r) -> Permutation (x :: l) (y :: r).
+Proof.
+  intros x l; revert x.
+  induction l; intros.
+  - simpl in *. inversion H. apply Permutation_refl.
+  - unfold select in H.  
+    bdestruct (x <=? a); fold select in H.
+    + specialize (IHl x).   
+      destruct (select x l) eqn:Seq.
+      apply perm_trans with (a :: n :: l0);
+        try apply perm_swap.
+      apply perm_trans with (a :: x :: l);
+        try apply perm_swap.
+      apply perm_skip.
+      apply IHl. reflexivity. inversion H. rewrite <- H2.
+      apply perm_swap.
+    + specialize (IHl a).
+      destruct (select a l) eqn:Seq.
+      apply perm_trans with (x :: n :: l0);
+        try apply perm_swap.
+      apply perm_skip. apply IHl.
+      reflexivity. inversion H. apply perm_swap.
+Qed.
+
+Lemma select_rest_length : forall x l y r, select x l = (y, r) -> list_length l = list_length r.
+Proof.
+  intros. apply select_perm in H.
+  apply Permutation_length in H. auto.
+Qed.
+
+Lemma selsort_perm: forall n l, list_length l = n -> Permutation l (selsort l n).
+Proof.
+  induction n.
+  - intros. rewrite length_zero_iff_nil in H.
+    subst. apply Permutation_refl.
+  - intros. destruct l. inversion H.
+    simpl. 
+    destruct (select n0 l) eqn:Seq.
+    apply perm_trans with (n1 :: l0).
+    apply select_perm. auto.
+    apply perm_skip. apply IHn. inversion H.
+    symmetry. eapply select_rest_length. eauto.
+    (* apply select_rest_length in Seq. auto. *)
+Qed.
+
+Lemma selection_sort_perm: forall l, Permutation l (selection_sort l).
+Proof. 
+  unfold selection_sort. intros. 
+  apply selsort_perm. reflexivity. 
+Qed.
+
+Lemma select_exists (l : list nat) (a : nat) : exists i j, select a l = (i ,j).
+Proof.
+  generalize dependent a. induction l.
+  - intros. exists a. exists []. reflexivity.
+  - intros. unfold select. destruct (a0 <=? a).
+  + fold select. assert (P: exists i j, select a0 l = (i,j)). apply IHl.
+  inversion P. inversion H. exists x. exists (a :: x0). rewrite H0. reflexivity.
+  + fold select. assert (P: exists i j, select a l = (i,j)). apply IHl.
+  inversion P. inversion H. exists x. exists (a0 :: x0). rewrite H0. reflexivity.
+Qed.
+
+Lemma select_fst_leq: forall al bl x y, select x al = (y, bl) -> y <= x.
+Proof.
+  intros. 
+  unfold select in H.
+  generalize dependent x; generalize dependent y; generalize dependent bl. induction al.
+  - intros. inversion H. auto.
+  - intros. fold select in IHal. fold select in H.  
+  bdestruct (x <=? a).
+  -- pose (select_exists al x).
+  inversion e. inversion H1. rewrite H2 in H. apply IHal with (bl := x1). inversion H. 
+  rewrite <- H4. auto.
+  -- pose (select_exists al a).
+  inversion e. inversion H1. rewrite H2 in H. inversion H. rewrite <- H4.
+  apply IHal in H2. inversion H2. unfold gt in H0. apply lt_n_Sm_le. apply lt_S. auto. 
+  unfold gt in H0. apply le_lt_n_Sm in H3. rewrite H6 in H3. assert (Q: x0 < x). 
+  apply lt_trans with (m := a). auto. auto. apply lt_n_Sm_le. apply lt_S. auto.
+Qed. 
+
+Definition le_all x xs := Forall (fun y => x <= y) xs.
+Hint Unfold le_all : core.
+Infix "<=*" := le_all (at level 70, no associativity).
+
+Lemma le_all__le_one : forall lst y n, y <=* lst -> In n lst -> y <= n.
+Proof. 
+  intros. unfold le_all in H. destruct H.
+  - contradiction.
+  - pose (select_perm n (x::l)). pose (select_exists (x::l) n). inversion e. inversion H2.
+  apply p in H3. apply in_inv in H0. destruct H0.
+  -- rewrite <- H0. auto.
+  -- rewrite Forall_forall in H1. apply H1. auto.
+Qed.
+
+(* I think this is a good example of where forward reasoning makes targeting lemmas easier *)
+Lemma select_smallest: forall al bl x y, select x al = (y, bl) -> y <=* bl.
+Proof.
+  intros. unfold le_all. 
+  generalize dependent bl; generalize dependent x; generalize dependent y. induction al.
+  - intros. inversion H. auto.
+  - intros. unfold select in H. bdestruct (x <=? a).
+  * fold select in H. pose (select_exists al x). inversion e. inversion H1.
+  rewrite H2 in H. inversion H2. apply IHal in H2. inversion H. apply Forall_cons.
+  ** apply le_trans with (m:=x). rewrite <- H5. eapply select_fst_leq. eauto. auto.
+  ** rewrite <- H5. auto.
+  * fold select in H. pose (select_exists al a). inversion e. inversion H1. rewrite H2 in H.
+  inversion H2.  apply IHal in H2. inversion H. apply Forall_cons.
+  ** rewrite <- H5. apply lt_n_Sm_le. apply lt_S. apply Nat.le_lt_trans with (m:=a). 
+  eapply select_fst_leq. eauto. auto.
+  ** rewrite <- H5. auto.
+Qed. 
+   
+Lemma select_in : forall al bl x y, select x al = (y, bl) -> In y (x :: al).
+Proof. intros.
+  generalize dependent bl; generalize dependent x; generalize dependent y. induction al.
+  - intros. inversion H. simpl. left. reflexivity.
+  - intros. 
+  * inversion H. bdestruct (x <=? a). 
+  ** simpl. apply or_comm. apply or_assoc. 
+  right. apply or_comm. replace (x = y \/ In y al) with (In y (x :: al)).
+  pose (select_exists al x). inversion e. inversion H2. rewrite H3 in H1. 
+  inversion H1. eapply IHal. rewrite <- H5. eauto. simpl. reflexivity.
+  ** apply select_perm in H. eapply Permutation_in. apply Permutation_sym. eauto. 
+  simpl. left. auto.
+Qed.
+
+Lemma cons_of_small_maintains_sort: forall bl y n,
+  n = list_length bl -> y <=* bl -> sorted (selsort bl n) -> sorted (y :: selsort bl n).
+Proof.
+  intros. symmetry in H. apply selsort_perm in H. induction (selsort bl n).
+  - apply sorted_1.
+  - apply sorted_cons. eapply le_all__le_one. eauto. eapply Permutation_in. 
+  apply Permutation_sym. eauto. simpl. auto. auto.
+Qed.
+
+Lemma selsort_sorted : forall n al, list_length al = n -> sorted (selsort al n).
+Proof.
+  intros. generalize dependent al. induction n.
+  - intros. assert (P : al = []). destruct al. auto. simpl in H. inversion H. 
+  rewrite P. simpl. apply sorted_nil.
+  - intros. destruct al. simpl in H. inversion H.
+  simpl in H. inversion H. simpl. pose (select_exists al n0).
+  inversion e. inversion H0.
+  rewrite H2. apply cons_of_small_maintains_sort.
+  + eapply select_rest_length. eauto.
+  + eapply select_smallest. eauto.
+  + rewrite H1. apply IHn. rewrite <- H1. symmetry. eapply select_rest_length. eauto.
+Qed. 
+
+Lemma selection_sort_sorted : forall al, sorted (selection_sort al).
+Proof.
+  unfold selection_sort. intros. apply selsort_sorted. reflexivity.
+Qed.
+
+Theorem selection_sort_is_correct : is_a_sorting_algorithm selection_sort.
+Proof.
+  unfold is_a_sorting_algorithm. intros. split.
+  apply selection_sort_perm. apply selection_sort_sorted.
+Qed.
+
+(* ################################################################# *)
+(** * Recursive Functions That are Not Structurally Recursive *)
+
+Require Import Recdef.  (* needed for [measure] feature *)
+
+Function selsortt l {measure list_length l} :=
+  match l with
+  | [] => []
+  | x :: r => let (y, r') := select x r
+            in y :: selsortt r'
+end.
+Proof.
+  intros l x r HL y r' Hsel.
+  apply select_rest_length in Hsel. inv Hsel. simpl. lia.
+Defined.
+
+Lemma selsortt_perm : forall n l, list_length l = n -> Permutation l (selsortt l).
+Proof.
+  induction n.
+  - intros. rewrite length_zero_iff_nil in H. subst. apply Permutation_refl.
+  - intros. destruct l. inversion H. rewrite selsortt_equation. 
+    destruct (select n0 l) eqn:Seq. apply perm_trans with (n1 :: l0).
+    + pose (select_perm n0 l). rewrite Seq in p. apply p. auto.
+    + apply perm_skip. apply IHn. simpl in H. inversion H. 
+    symmetry. eapply select_rest_length. eauto.
+    (* This is how dude from GitHub did it below *)
+    (* + apply perm_skip. apply IHn. assert (length (n0::l) = (length (n1::l0))).
+    { 
+      apply Permutation_length.
+      pose (select_perm n0 l).
+      rewrite Seq in p.
+      apply p. auto.
+    } inversion H0. inversion H. reflexivity. *)
+  Qed.
+
+Lemma list_has_length {T} (l : list T): exists x, list_length l = x.
+Proof. induction l. exists 0. reflexivity. inversion IHl. exists (S x). simpl. auto.
+Qed.
+
+Lemma cons_of_small_maintains_sortt: forall bl y,
+    y <=* bl -> sorted (selsortt bl) -> sorted (y :: selsortt bl).
+Proof. 
+  intros. assert (L: exists x, list_length bl = x). apply list_has_length.
+  inversion L. apply selsortt_perm in H1. induction (selsortt bl).
+  - apply sorted_1.
+  - apply sorted_cons. eapply le_all__le_one. eauto. eapply Permutation_in. 
+  apply Permutation_sym. eauto. simpl. auto. auto.
+Qed.
+
+Lemma selsortt_sorted : forall n al, list_length al = n -> sorted (selsortt al).
+Proof. 
+  intros. generalize dependent al. induction n.
+  - intros. assert (P : al = []). destruct al. auto. simpl in H. inversion H. 
+  rewrite P. simpl. apply sorted_nil.
+  - intros. destruct al. simpl in H. inversion H.
+  simpl in H. inversion H. simpl. pose (select_exists al n0).
+  inversion e. inversion H0. rewrite selsortt_equation. rewrite H2. apply cons_of_small_maintains_sortt.
+  + eapply select_smallest. eauto.
+  + apply IHn. rewrite <- H1. symmetry. eapply select_rest_length. eauto.
+Qed. 
+
+Theorem selsortt_is_correct :
+  is_a_sorting_algorithm selsortt.
+Proof. 
+  unfold is_a_sorting_algorithm. intros. assert (E: exists x, list_length al = x). apply list_has_length.
+  inversion E. split.
+  lfind_debug.
+  Admitted.
+
+  (* eapply selsortt_perm. eauto.
+  eapply selsortt_sorted. eauto.
+Qed. *)
