Selection/benchmarks/sources/selection_lemma_select_fst_leq_1_IN_select_smallest/Selection.v
@@ -1,0 +1,167 @@
+(** * Selection:  Selection Sort *)
+(* Some proofs from: https://github.com/kolya-vasiliev/verified-functional-algorithms-2019/blob/master/Selection.v *)
+
+Load LFindLoad.
+From lfind Require Import LFind.
+Unset Printing Notations.
+Set Printing Implicit.
+
+Set Warnings "-notation-overridden,-parsing,-deprecated-hint-without-locality".
+From VFA Require Import Perm.
+Hint Constructors Permutation : core.
+From Coq Require Export Lists.List.  (* for exercises involving [List.length] *)
+
+Definition list_length {T} (l : list T) := List.length l.
+
+(* ################################################################# *)
+(** * The Selection-Sort Program  *)
+Fixpoint select (x: nat) (l: list nat) : nat * list nat :=
+  match l with
+  | [] => (x, [])
+  | h :: t =>
+    if x <=? h
+    then let (j, l') := select x t
+         in (j, h :: l')
+    else let (j, l') := select h t
+         in (j, x :: l')
+  end.
+
+Fixpoint selsort (l : list nat) (n : nat) : list nat :=
+  match l, n with
+  | _, O => []  (* ran out of fuel *)
+  | [], _ => []
+  | x :: r, S n' => let (y, r') := select x r
+                  in y :: selsort r' n'
+end.
+
+Definition selection_sort (l : list nat) : list nat :=
+  selsort l (length l).
+  
+(* ################################################################# *)
+(** * Proof of Correctness *)
+
+Inductive sorted: list nat -> Prop :=
+ | sorted_nil: sorted []
+ | sorted_1: forall i, sorted [i]
+ | sorted_cons: forall i j l, i <= j -> sorted (j :: l) -> sorted (i :: j :: l).
+
+Hint Constructors sorted : core.
+
+Definition is_a_sorting_algorithm (f: list nat -> list nat) := forall al,
+    Permutation al (f al) /\ sorted (f al).
+
+Lemma select_perm: forall x l y r, select x l = (y, r) -> Permutation (x :: l) (y :: r).
+Proof.
+  intros x l; revert x.
+  induction l; intros.
+  - simpl in *. inversion H. apply Permutation_refl.
+  - unfold select in H.  
+    bdestruct (x <=? a); fold select in H.
+    + specialize (IHl x).   
+      destruct (select x l) eqn:Seq.
+      apply perm_trans with (a :: n :: l0);
+        try apply perm_swap.
+      apply perm_trans with (a :: x :: l);
+        try apply perm_swap.
+      apply perm_skip.
+      apply IHl. reflexivity. inversion H. rewrite <- H2.
+      apply perm_swap.
+    + specialize (IHl a).
+      destruct (select a l) eqn:Seq.
+      apply perm_trans with (x :: n :: l0);
+        try apply perm_swap.
+      apply perm_skip. apply IHl.
+      reflexivity. inversion H. apply perm_swap.
+Qed.
+
+Lemma select_rest_length : forall x l y r, select x l = (y, r) -> list_length l = list_length r.
+Proof.
+  intros. apply select_perm in H.
+  apply Permutation_length in H. auto.
+Qed.
+
+Lemma selsort_perm: forall n l, list_length l = n -> Permutation l (selsort l n).
+Proof.
+  induction n.
+  - intros. rewrite length_zero_iff_nil in H.
+    subst. apply Permutation_refl.
+  - intros. destruct l. inversion H.
+    simpl. 
+    destruct (select n0 l) eqn:Seq.
+    apply perm_trans with (n1 :: l0).
+    apply select_perm. auto.
+    apply perm_skip. apply IHn. inversion H.
+    symmetry. eapply select_rest_length. eauto.
+    (* apply select_rest_length in Seq. auto. *)
+Qed.
+
+Lemma selection_sort_perm: forall l, Permutation l (selection_sort l).
+Proof. 
+  unfold selection_sort. intros. 
+  apply selsort_perm. reflexivity. 
+Qed.
+
+Lemma select_exists (l : list nat) (a : nat) : exists i j, select a l = (i ,j).
+Proof.
+  generalize dependent a. induction l.
+  - intros. exists a. exists []. reflexivity.
+  - intros. unfold select. destruct (a0 <=? a).
+  + fold select. assert (P: exists i j, select a0 l = (i,j)). apply IHl.
+  inversion P. inversion H. exists x. exists (a :: x0). rewrite H0. reflexivity.
+  + fold select. assert (P: exists i j, select a l = (i,j)). apply IHl.
+  inversion P. inversion H. exists x. exists (a0 :: x0). rewrite H0. reflexivity.
+Qed.
+
+Lemma select_fst_leq: forall al bl x y, select x al = (y, bl) -> y <= x.
+Proof.
+  intros. 
+  unfold select in H.
+  generalize dependent x; generalize dependent y; generalize dependent bl. induction al.
+  - intros. inversion H. auto.
+  - intros. fold select in IHal. fold select in H.  
+  bdestruct (x <=? a).
+  -- pose (select_exists al x).
+  inversion e. inversion H1. rewrite H2 in H. apply IHal with (bl := x1). inversion H. 
+  rewrite <- H4. auto.
+  -- pose (select_exists al a).
+  inversion e. inversion H1. rewrite H2 in H. inversion H. rewrite <- H4.
+  apply IHal in H2. inversion H2. unfold gt in H0. apply lt_n_Sm_le. apply lt_S. auto. 
+  unfold gt in H0. apply le_lt_n_Sm in H3. rewrite H6 in H3. assert (Q: x0 < x). 
+  apply lt_trans with (m := a). auto. auto. apply lt_n_Sm_le. apply lt_S. auto.
+Qed. 
+
+Definition le_all x xs := Forall (fun y => x <= y) xs.
+Hint Unfold le_all : core.
+Infix "<=*" := le_all (at level 70, no associativity).
+
+Lemma le_all__le_one : forall lst y n, y <=* lst -> In n lst -> y <= n.
+Proof. 
+  intros. unfold le_all in H. destruct H.
+  - contradiction.
+  - pose (select_perm n (x::l)). pose (select_exists (x::l) n). inversion e. inversion H2.
+  apply p in H3. apply in_inv in H0. destruct H0.
+  -- rewrite <- H0. auto.
+  -- rewrite Forall_forall in H1. apply H1. auto.
+Qed.
+
+(* I think this is a good example of where forward reasoning makes targeting lemmas easier *)
+Lemma select_smallest: forall al bl x y, select x al = (y, bl) -> y <=* bl.
+Proof.
+  intros. unfold le_all. 
+  generalize dependent bl; generalize dependent x; generalize dependent y. induction al.
+  - intros. inversion H. auto.
+  - intros. unfold select in H. bdestruct (x <=? a).
+  * fold select in H. pose (select_exists al x). inversion e. inversion H1.
+  rewrite H2 in H. inversion H2. apply IHal in H2. inversion H. apply Forall_cons.
+  ** apply le_trans with (m:=x). rewrite <- H5. 
+  lfind_debug.
+  Admitted.
+  
+  (* eapply select_fst_leq. eauto. auto.
+  ** rewrite <- H5. auto.
+  * fold select in H. pose (select_exists al a). inversion e. inversion H1. rewrite H2 in H.
+  inversion H2.  apply IHal in H2. inversion H. apply Forall_cons.
+  ** rewrite <- H5. apply lt_n_Sm_le. apply lt_S. apply Nat.le_lt_trans with (m:=a). 
+  eapply select_fst_leq. eauto. auto.
+  ** rewrite <- H5. auto.
+Qed.  *)
